{-# OPTIONS --without-K --exact-split --safe #-}

module TypeTheory.Negation where

open import TypeTheory.Universes
open import TypeTheory.SimpleTypes
open import TypeTheory.Product
open import TypeTheory.Sum
open import HoTT.Identity-Types
open import TypeTheory.LogicalEquiv

--------------------------------------
-- logical negation

not : Type ð‘¢ -> Type ð‘¢
not X = X -> Zero

-- double negation
not-not : Type ð‘¢ -> Type ð‘¢
not-not A = not (not A) -- (A -> 0) -> 0

-- tripple negation
not-not-not : Type ð‘¢ -> Type ð‘¢
not-not-not A = not (not-not A)

-- double negation introduction A => Â¬Â¬A
not-not-intro : {A : Type ð‘¢} -> A -> not-not A
not-not-intro a absurdA = absurdA a

-- if we have function A->B and B is empty B -> 0
-- then A is empty A -> 0
contrapositive : {A : Type ð‘¢} {B : Type ð‘¤}
                 -> (A -> B)
                 -> not B -> not A
contrapositive f b->0 a = b->0 (f a)

-- absurdity of absurdity of absurdity is absurdity
not-not-not-A-imply-not-A : {A : Type ð‘¢}
                         -> not (not (not A))
                         -> not A
not-not-not-A-imply-not-A nnna = contrapositive not-not-intro nnna

not-not-not-intro : {A : Type ð‘¢}
                 -> not A
                 -> not (not (not A))
not-not-not-intro nA = not-not-intro nA

absurdity^3-is-absurdity : {A : Type ð‘¢}
                           -> not (not (not A)) <=> not A
absurdity^3-is-absurdity {u} {X} =
  ( firstly ,, secondly )
  where
   firstly : not (not (not X)) -> not X
   firstly = not-not-not-A-imply-not-A
   secondly : not X -> not (not (not X))
   secondly = not-not-not-intro

1-is-not-empty : not (is-empty One)
1-is-not-empty f = f <>

----------------------------------
-- negation of Identity types
-- x1 â‰¡ x2 -> 0
-- inequality "x1 is not equal to x2 in type X"
_â‰¡/_ : {X : Type ð‘¢} -> X -> X -> Type ð‘¢
x1 â‰¡/ x2 = not (x1 â‰¡ x2)

-- swap
â‰¡/-sym : {A : Type ð‘¢} {x y : A} -> x â‰¡/ y -> y â‰¡/ x
â‰¡/-sym  {U} {A} {x} {y} x-noâ‰¡-y = \ yâ‰¡x -> x-noâ‰¡-y (â‰¡-swap (yâ‰¡x)) -- (y â‰¡ x) -> Zero

{-- not transitive a â‰¡/ b, b â‰¡/ a but a â‰¡ a
â‰¡/-not-trans : {A : Type ð‘¢} {x y z : A} -> not ( x â‰¡/ y -> y â‰¡/ z -> x â‰¡/ z )
â‰¡/-not-trans a = {!   !}
-}

One-is-not-Zero : One â‰¡/ Zero
One-is-not-Zero 1=0 = â‰¡->Fun 1=0 <>

right-fails-gives-left-holds : {P : Type ð‘¢} {Q : Type ð‘¤}
                          -> (P + Q) -> (not Q) -> P
right-fails-gives-left-holds (left p) u = p
right-fails-gives-left-holds (right q) u = absurd _ (u q)
